\documentclass{article}

\title{Complex Variables Homework Section 21}
\author{Adam Buskirk}

\usepackage{amssymb,amsmath,amsthm}
\usepackage{tikz}
\usepackage[margin=1in]{geometry}

\newtheorem{theorem}[subsection]{Theorem}
\newtheorem{conjecture}[subsection]{Conjecture}
\newtheorem{lemma}[subsection]{Lemma}
\theoremstyle{definition}
\newtheorem{definition}[subsection]{Definition}

\newcommand{\R}{\mathbb{R}}
\newcommand{\N}{\mathbb{N}}
\newcommand{\Q}{\mathbb{Q}}
\newcommand{\Z}{\mathbb{Z}}
\newcommand{\Co}{\mathbb{C}}
\newcommand{\p}[1]{\left(#1\right)}
\newcommand{\sq}[1]{\left[#1\right]}
\newcommand{\set}[1]{\left\{#1\right\}}
\newcommand{\norm}[1]{\left|\left|#1\right|\right|}
% \newcommand{\p}[1]{\left(#1\right)}

\begin{document}
\maketitle
p. 71 \#1 bd [Verify the C-R equations for f(x)=1/z].

\section{Problem 1}
\subsection{Part b}
For $f(z) = z-\bar{z}$, 
\[ u(x,y) = 0 \qquad v(x,y) = 2y \]
So $v_y = 2 \neq 0 = u_x$, contradicting the first equation in (7) in the text.

\subsection{Part d}
For $f(z)=e^x e^{-iy}$,
\[ u(x,y) = e^x \cos(-y) = e^x \cos(y) \]
\[ v(x,y) = e^x \sin(-y) = -e^x \sin(y) \]
Thus
\[ u_x = e^x \cos(y) \]
\[ u_y = -e^x \sin(y) \]
\[ v_x = -e^x \sin(y) \]
\[ v_y = -e^x \cos(y) \]

But
\[ u_y = -e^x \sin y \neq -\sq{ -e^x \sin y} = -v_x \]
Unless, per chance, $y \in \pi\Z$. In this case, however, $\cos(y) \neq 0$,
which means the second condition,
\[ u_x = e^x \cos(y) \neq -e^x \cos(y) = v_y \]
cannot be satisfied. Hence $f$ is not differentiable at any point.

\section{Verify C-R}
For $f(z)=1/z$,
\[ u(x,y) = \frac{x}{x^2+y^2} \]
\[ v(x,y) = \frac{-y}{x^2+y^2} \]
Thus 
\[ 
u_x 
= \frac{d}{dx} \sq{ x(x^2+y^2)^{-1} }
= \frac{1}{x^2+y^2} + x (-1) (x^2+y^2)^{-2} (2x) 
= \frac{1}{x^2+y^2} - \frac{ 2x^2 }{(x^2+y^2)^2}
\]
\[
= \frac{x^2+y^2 - 2x^2}{(x^2+y^2)^2}
= \frac{y^2-x^2}{(x^2+y^2)^2}
\]
and
\[
u_y
= \frac{d}{dy} \sq{x (x^2+y^2)^{-1} }
= x D_y \sq{ (x^2+y^2)^{-1} }
= x \sq{(-1) (x^2+y^2)^{-2} 2y}
= \frac{-2xy}{(x^2+y^2)^{2}}
\]
and
\[
v_x 
= D_x \sq{-y (x^2+y^2)^{-1}}
= -y D_x (x^2+y^2)^{-1}
= -y (-1) (x^2+y^2)^{-2} 2x
= \frac{2xy}{(x^2+y^2)^{2}}
\]
and 
\[
v_y
= D_y \sq{ -y (x^2+y^2)^{-1} }
= - \sq{1 \cdot (x^2+y^2)^{-1} + y (-1) (x^2+y^2)^{-2} (2y) }
= - \sq{\frac{1}{x^2+y^2} - \frac{2y^2}{(x^2+y^2)^2}  }
\]
\[
= - \frac{x^2+y^2 - 2y^2}{(x^2+y^2)^2}
= - \frac{x^2-y^2}{(x^2+y^2)^2}
= \frac{y^2-x^2}{(x^2+y^2)^2}
\]

From these, it is evident that
\[
u_x = \frac{y^2-x^2}{(x^2+y^2)^2} = v_y 
\]
and
\[ 
u_y = \frac{-2xy}{(x^2+y^2)^2} = -\p{\frac{2xy}{(x^2+y^2)^2}} = -v_x
\]
and thus $f(x) = 1/z$ satisfies the Caucy-Riemann equations.


\end{document}
