\documentclass{article}

\title{Complex Variables Homework Section 33}
\author{Adam Buskirk}

\usepackage{amssymb,amsmath,amsthm}
\usepackage{tikz}
\usepackage[margin=1in]{geometry}

\newtheorem{theorem}[subsection]{Theorem}
\newtheorem{conjecture}[subsection]{Conjecture}
\newtheorem{lemma}[subsection]{Lemma}
\theoremstyle{definition}
\newtheorem{definition}[subsection]{Definition}

\newcommand{\R}{\mathbb{R}}
\newcommand{\N}{\mathbb{N}}
\newcommand{\Q}{\mathbb{Q}}
\newcommand{\Z}{\mathbb{Z}}
\newcommand{\Co}{\mathbb{C}}
\newcommand{\p}[1]{\left(#1\right)}
\newcommand{\sq}[1]{\left[#1\right]}
\newcommand{\set}[1]{\left\{#1\right\}}
\newcommand{\abs}[1]{\left|#1\right|}
\newcommand{\norm}[1]{\left|\left|#1\right|\right|}
% \newcommand{\p}[1]{\left(#1\right)}
\allowdisplaybreaks[1]

\begin{document}
\maketitle

\section{Problem 1}
Find $(-1)^{1/3}$ and PV $(-1)^{1/3}$.

\begin{align*}
(-1)^{1/3} 
&= e^{1/3 \log (-1)} \\
&= e^{1/3 (\ln 1 + i (\pi + 2 \pi n))} \\
&= e^{1/3 (i (\pi + 2 \pi n))} \\
&= e^{i \pi /3 + 2/3 i \pi n} \\
&= e^{i (\pi/3 + 2/3 \pi n)} \\
&= \cos\p{\frac{\pi}{3} + \frac{2}{3} \pi n} 
+ i \sin\p{\frac{\pi}{3} + \frac{2}{3} \pi n}
\end{align*}

In particular, the principal value of $(-1)^{1/3}$ is $0.5+\sqrt{3}/2$.

\section{Problem 2}
\begin{lemma}
\[ \overline{e^{z}} = e^{\bar{z}} \]
\end{lemma}
\begin{proof}
Let $x+yi=z$.
\begin{align*}
\overline{e^z}
&= \overline{e^x} e^{yi} \\
&= \overline{e^x \p{\cos(y)+i\sin(y)}} \\
&= e^x \overline{\p{\cos y + i \sin y}} \\
&= e^x \p{\cos y - i \sin y } \\
&= e^x \p{ \cos (-y) + i \sin (-y) } \\
&= e^x e^{i(-y)} \\
&= e^{x-yi} \\
&= e^{\bar{z}}
\end{align*}
\end{proof}

\begin{theorem}
\[\overline{\sin(z)} = \sin(\bar{z})\]
\end{theorem}
\begin{proof}
\begin{align*}
\overline{\sin(z)}
&= \overline{\p{\frac{e^{iz}-e^{-iz}}{2i}}} \\
&= \frac{\p{\overline{e^{iz}-e^{-iz}}}}{\overline{2i}} \\
&= \frac{ \overline{e^{iz}} - \overline{e^{-iz}} }{-2i} \\
&= \frac{ e^{(\overline{iz})} - e^{(\overline{-iz})} }{-2i} \\
&= \frac{ e^{\bar{i} \bar{z}} - e^{\overline{-i}\bar{z}} }{-2i} \\
&= \frac{ e^{-i \bar{z}} - e^{i\bar{z}} }{-2i} \\
&= \frac{   e^{i\bar{z}} - e^{-i \bar{z}}}{2i} \\
&= \sin(\bar{z})
\end{align*}
\end{proof}

\end{document}
