\documentclass{article}

\title{Complex Variables Section 26 Homework}
\author{Adam Buskirk}

\usepackage{amssymb,amsmath,amsthm}
\usepackage{tikz}
\usepackage[margin=1in]{geometry}

\newtheorem{theorem}[subsection]{Theorem}
\newtheorem{conjecture}[subsection]{Conjecture}
\newtheorem{lemma}[subsection]{Lemma}
\theoremstyle{definition}
\newtheorem{definition}[subsection]{Definition}

\newcommand{\R}{\mathbb{R}}
\newcommand{\N}{\mathbb{N}}
\newcommand{\Q}{\mathbb{Q}}
\newcommand{\Z}{\mathbb{Z}}
\newcommand{\Co}{\mathbb{C}}
\newcommand{\p}[1]{\left(#1\right)}
\newcommand{\sq}[1]{\left[#1\right]}
\newcommand{\set}[1]{\left\{#1\right\}}
\newcommand{\norm}[1]{\left|\left|#1\right|\right|}
% \newcommand{\p}[1]{\left(#1\right)}
\allowdisplaybreaks[1]

\begin{document}
\maketitle

\begin{quote}
Find harmonic conjugates for
\[ u(x,y) = \frac{x}{x^2+y^2} \]
and
\[ u(x,y) = \ln \sqrt{x^2+y^2} \]
\end{quote}

For the first,
\begin{align*}
u_x
&= D_x x (x^2+y^2)^{-1} \\
&= (x^2+y^2)^{-1} + x (-1) (x^2+y^2)^{-2} (2x) \\
&= \frac{1}{x^2+y^2} - \frac{2x^2}{(x^2+y^2)^2} \\
&= \frac{x^2+y^2 - 2x^2}{(x^2+y^2)^2} \\
&= \frac{y^2-x^2}{x^2+y^2} \\
u_y
&= D_y x (x^2+y^2)^{-1} \\
&= x (-1) (x^2+y^2)^{-2} 2y \\
&= - \frac{2xy}{(x^2+y^2)^2} 
\end{align*}

Thus, for a harmonic conjugate $v$,
\begin{align*}
v_x
&= \frac{2xy}{(x^2+y^2)^2} \\
\int v_x \;dx 
&= \int \frac{2xy}{(x^2+y^2)^2} \;dx \\
&= \int 2xy (x^2+y^2)^{-2} \;dx \\
&= \int 2x \frac{ D_x y(x^2+y^2)^{-1} }{-2x} \;dx \\
&= - \int D_x y(x^2+y^2) \;dx \\
&= - \frac{y}{x^2+y^2} + C(y) \\
v_y
&= \frac{y^2-x^2}{(x^2+y^2)^2} \\
\int v_y \;dy 
&=  \int \frac{y^2 - x^2}{(x^2+y^2)^2} \;dy \\
&= -\int \frac{x^2 - y^2}{(x^2+y^2)^2} \;dy \\
&= -\int \frac{x^2 + y^2}{(x^2+y^2)^2} + \frac{-2y^2}{(x^2+y^2)^2} \;dy \\
&= -\int \frac{1}{x^2+y^2} + \frac{-2y^2}{(x^2+y^2)^2} \;dy \\
&= -\int \sq{D_y y} (x^2+y^2)^{-1} + y (2y) (-1) (x^2+y^2)^{-2} \;dy \\
&= -\int \sq{D_y y} (x^2+y^2)^{-1} + y \sq{D_y (x^2+y^2)^{-1}} \;dy \\
&= -\int D_y \sq{y (x^2+y^2)^{-1}} \;dy \\
&= -\frac{y}{x^2+y^2} + C(x)
\end{align*}
Thus, the function 
\[ v(x,y) = \frac{-y}{x^2+y^2} \]
is a harmonic conjugate to $u$ defined above.

For the second problem,
\[ u(x,y) = \ln \sqrt{x^2+y^2} \]
\begin{align*}
u_x 
&= \frac{1}{\sqrt{x^2+y^2}} 
\cdot \frac{1}{2} \frac{1}{\sqrt{x^2+y^2}}
\cdot 2x \\
&= \frac{x}{x^2 + y^2} \\
u_y
&= \frac{1}{\sqrt{x^2+y^2}} 
\cdot \frac{1}{2} \frac{1}{\sqrt{x^2+y^2}}
\cdot 2y \\
&= \frac{y}{x^2 + y^2} \\
v_x &= -u_y \\
&= - \frac{y}{x^2+y^2} \\
v
&=\int v_x \;dx \\
&= \int -\frac{y}{x^2+y^2} \;dx \\
&= - y \int \frac{1}{x^2+y^2} \;dx \\
&= - y \sq{\frac{1}{y} \tan^{-1} \frac{x}{y}} +C(y) \\
&= - \tan^{-1} \frac{x}{y} + C(y)\\
&= \tan^{-1} \frac{y}{x} + \frac{\pi}{2} + C(y) \\
v_y &= u_x \\
&= \frac{x}{x^2+y^2} \\
v
&= \int \frac{x}{x^2+y^2} \;dy \\
&= x \int \frac{1}{x^2+y^2} \;dy \\
&= x \sq{ \frac{1}{x}\tan^{-1} \frac{y}{x} + C(x)} \\
&= \tan^{-1} \frac{y}{x} + C(x) \\
\end{align*}
Observe that these two conditions are satisfied if $C(x)=\pi/2$ and $C(y)=0$. 
Thus $(u,v)$ is a harmonic conjugate pair for $v(x,y)=\tan^{-1} (y/x)+\pi/2$.

\end{document}
